BoogieLang/Util.thy
@@ -3,25 +3,25 @@ imports Semantics "HOL-Eisbach.Eisbach" "HOL-Eisbach.Eisbach_Tools"
 begin
 
 lemma assert_correct:
-  "\<lbrakk>\<Lambda>,\<Gamma> \<turnstile> \<langle>Assert e, Normal n_s\<rangle> \<rightarrow> s; \<Gamma> \<turnstile> \<langle>e, n_s\<rangle> \<Down> (BoolV True) \<rbrakk> \<Longrightarrow> s = Normal n_s"
+  "\<lbrakk>A,\<Lambda>,\<Gamma> \<turnstile> \<langle>Assert e, Normal n_s\<rangle> \<rightarrow> s; A,\<Gamma> \<turnstile> \<langle>e, n_s\<rangle> \<Down> LitV (LBool True) \<rbrakk> \<Longrightarrow> s = Normal n_s"
   by (erule red_cmd.cases; simp; blast dest: expr_eval_determ(1))
 
 (*TODO, rewrite this as an elimination rule to be consistent with other rules *)
 lemma assert_correct_2:
-  "\<lbrakk>\<Lambda>,\<Gamma> \<turnstile> \<langle>Assert e, s\<rangle> \<rightarrow> s'; s = Normal n_s; \<Gamma> \<turnstile> \<langle>e, n_s\<rangle> \<Down> (BoolV True)\<rbrakk> \<Longrightarrow> s' = Normal n_s"
+  "\<lbrakk>A,\<Lambda>,\<Gamma> \<turnstile> \<langle>Assert e, s\<rangle> \<rightarrow> s'; s = Normal n_s; A,\<Gamma> \<turnstile> \<langle>e, n_s\<rangle> \<Down> LitV (LBool True)\<rbrakk> \<Longrightarrow> s' = Normal n_s"
   by (erule red_cmd.cases; simp; blast dest: expr_eval_determ(1))
 
 lemma assert_ml: 
-"\<lbrakk> \<Lambda>, \<Gamma> \<turnstile> \<langle>(Assert e) # cs, Normal ns\<rangle> [\<rightarrow>] s';
-  \<Gamma> \<turnstile> \<langle>e, ns\<rangle> \<Down> BoolV True;
-  \<Lambda>, \<Gamma> \<turnstile> \<langle>cs, Normal ns\<rangle> [\<rightarrow>] s' \<Longrightarrow> P \<rbrakk> \<Longrightarrow> P"
+"\<lbrakk> A,\<Lambda>,\<Gamma> \<turnstile> \<langle>(Assert e) # cs, Normal ns\<rangle> [\<rightarrow>] s';
+  A,\<Gamma> \<turnstile> \<langle>e, ns\<rangle> \<Down> LitV (LBool True);
+  A,\<Lambda>,\<Gamma> \<turnstile> \<langle>cs, Normal ns\<rangle> [\<rightarrow>] s' \<Longrightarrow> P \<rbrakk> \<Longrightarrow> P"
   apply (erule RedCmdListCons_case)
   by (blast dest: assert_correct)
 
 lemma assert_true_cmds: 
-"\<lbrakk> \<Lambda>, \<Gamma> \<turnstile> \<langle>(Assert (Val (BoolV True))) # cs, Normal ns\<rangle> [\<rightarrow>] s';
-  \<Lambda>, \<Gamma> \<turnstile> \<langle>cs, Normal ns\<rangle> [\<rightarrow>] s' \<Longrightarrow> P \<rbrakk> \<Longrightarrow> P"
-  by (auto intro: RedVal elim: assert_ml)
+"\<lbrakk> A,\<Lambda>,\<Gamma> \<turnstile> \<langle>(Assert (Lit (LBool True))) # cs, Normal ns\<rangle> [\<rightarrow>] s';
+  A,\<Lambda>,\<Gamma> \<turnstile> \<langle>cs, Normal ns\<rangle> [\<rightarrow>] s' \<Longrightarrow> P \<rbrakk> \<Longrightarrow> P"
+  by (auto intro: RedLit elim: assert_ml)
 
 lemma imp_conj_assoc: "(A \<and> B) \<and> C \<longrightarrow> D \<Longrightarrow> A \<and> (B \<and> C) \<longrightarrow> D"
   by simp
@@ -48,102 +48,109 @@ lead to non-terminating tactics most likely due to \<Gamma> ''f'' appearing on b
 definition opaque_comp 
   where "opaque_comp f g x = f (g x)"
 
-lemma axioms_sat_mem: "a \<in> set(as) \<Longrightarrow> axioms_sat \<Gamma> ns as \<Longrightarrow> \<Gamma> \<turnstile> \<langle>a, ns\<rangle> \<Down> BoolV (True)"
+lemma axioms_sat_mem: "a \<in> set(as) \<Longrightarrow> axioms_sat A \<Gamma> ns as \<Longrightarrow> A,\<Gamma> \<turnstile> \<langle>a, ns\<rangle> \<Down> LitV (LBool (True))"
  by (simp add: axioms_sat_def axiom_sat_def list_all_iff)
 
 lemma assume_cases_2: 
-  "\<lbrakk>\<Lambda>,\<Gamma> \<turnstile> \<langle>Assume e, Normal n_s\<rangle> \<rightarrow> s; 
+  "\<lbrakk>A,\<Lambda>,\<Gamma> \<turnstile> \<langle>Assume e, Normal n_s\<rangle> \<rightarrow> s; 
     s = Magic \<Longrightarrow> P; 
     s = Normal n_s \<Longrightarrow> P \<rbrakk> \<Longrightarrow> P"
   by (erule red_cmd.cases; simp)
 
 lemma assume_cases_ext: 
-  "\<lbrakk>\<Lambda>,\<Gamma> \<turnstile> \<langle>Assume e, Normal n_s\<rangle> \<rightarrow> s; 
+  "\<lbrakk>A,\<Lambda>,\<Gamma> \<turnstile> \<langle>Assume e, Normal n_s\<rangle> \<rightarrow> s; 
     s = Magic \<Longrightarrow> P; 
-    s = Normal n_s \<Longrightarrow> \<Gamma> \<turnstile> \<langle>e, n_s\<rangle> \<Down> (BoolV True) \<Longrightarrow> P \<rbrakk> \<Longrightarrow> P"
+    s = Normal n_s \<Longrightarrow> A,\<Gamma> \<turnstile> \<langle>e, n_s\<rangle> \<Down> LitV (LBool True) \<Longrightarrow> P \<rbrakk> \<Longrightarrow> P"
   by (erule red_cmd.cases; simp)
 
 lemma assume_cases_ext_2: 
-  "\<lbrakk>\<Lambda>,\<Gamma> \<turnstile> \<langle>Assume e, s\<rangle> \<rightarrow> s'; 
+  "\<lbrakk>A,\<Lambda>,\<Gamma> \<turnstile> \<langle>Assume e, s\<rangle> \<rightarrow> s'; 
     s = Normal n_s;
     s' = Magic \<Longrightarrow> P; 
-    s' = Normal n_s \<Longrightarrow> \<Gamma> \<turnstile> \<langle>e, n_s\<rangle> \<Down> (BoolV True) \<Longrightarrow>  P \<rbrakk> \<Longrightarrow> P"
+    s' = Normal n_s \<Longrightarrow> A,\<Gamma> \<turnstile> \<langle>e, n_s\<rangle> \<Down> LitV (LBool True) \<Longrightarrow>  P \<rbrakk> \<Longrightarrow> P"
   by (erule red_cmd.cases; simp)
 
 lemma assume_ml: 
-  "\<lbrakk>\<Lambda>, \<Gamma> \<turnstile> \<langle>(Assume e) # cs, Normal ns\<rangle> [\<rightarrow>] s';
+  "\<lbrakk>A,\<Lambda>,\<Gamma> \<turnstile> \<langle>(Assume e) # cs, Normal ns\<rangle> [\<rightarrow>] s';
        s' = Magic \<Longrightarrow> P;
-        \<Gamma> \<turnstile> \<langle>e, ns\<rangle> \<Down> (BoolV True) \<Longrightarrow> \<Lambda>, \<Gamma> \<turnstile> \<langle>cs, Normal ns\<rangle> [\<rightarrow>] s' \<Longrightarrow> P\<rbrakk> \<Longrightarrow> P"
+        A,\<Gamma> \<turnstile> \<langle>e, ns\<rangle> \<Down> LitV (LBool True) \<Longrightarrow> A,\<Lambda>,\<Gamma> \<turnstile> \<langle>cs, Normal ns\<rangle> [\<rightarrow>] s' \<Longrightarrow> P\<rbrakk> \<Longrightarrow> P"
   apply (erule RedCmdListCons_case)
   by (metis assume_cases_ext magic_stays_cmd_list)
 
 lemma assume_false_cmds:
-  "\<lbrakk>\<Lambda>, \<Gamma> \<turnstile> \<langle>(Assume (Val (BoolV False))) # cs, Normal ns\<rangle> [\<rightarrow>] s';
+  "\<lbrakk>A,\<Lambda>,\<Gamma> \<turnstile> \<langle>(Assume (Lit (LBool False))) # cs, Normal ns\<rangle> [\<rightarrow>] s';
        s' = Magic \<Longrightarrow> P\<rbrakk> \<Longrightarrow> P"
   apply (erule RedCmdListCons_case)
-  by (metis RedVal assume_cases_ext expr_eval_determ(1) magic_stays_cmd_list val.inject(1))
+  by (metis RedAssertFail RedLit assert_correct assume_cases_ext magic_stays_cmd_list state.distinct(1))
+
+  (*by (metis RedLit assume_cases_ext expr_eval_determ(1) magic_stays_cmd_list val.inject(1))*)
 
 lemma assume_true_cmds: 
-  "\<lbrakk>\<Lambda>, \<Gamma> \<turnstile> \<langle>(Assume e) # cs, Normal ns\<rangle> [\<rightarrow>] s';
+  "\<lbrakk>A,\<Lambda>,\<Gamma> \<turnstile> \<langle>(Assume e) # cs, Normal ns\<rangle> [\<rightarrow>] s';
        s' = Magic \<Longrightarrow> P;
-       \<Lambda>, \<Gamma> \<turnstile> \<langle>cs, Normal ns\<rangle> [\<rightarrow>] s' \<Longrightarrow> P\<rbrakk> \<Longrightarrow> P"
+       A,\<Lambda>,\<Gamma> \<turnstile> \<langle>cs, Normal ns\<rangle> [\<rightarrow>] s' \<Longrightarrow> P\<rbrakk> \<Longrightarrow> P"
   by (rule assume_ml)
 
 lemma single_assign_cases:
-  "\<lbrakk>\<Lambda>,\<Gamma> \<turnstile> \<langle>Assign [(x,e)], s\<rangle> \<rightarrow> s'; 
+  "\<lbrakk>A,\<Lambda>,\<Gamma> \<turnstile> \<langle>Assign [(x,e)], s\<rangle> \<rightarrow> s'; 
    s = Normal n_s;
-   \<And>v. \<Gamma> \<turnstile> \<langle>e, n_s\<rangle> \<Down> v \<Longrightarrow> s' = Normal (n_s(x \<mapsto> v)) \<Longrightarrow> P \<rbrakk> \<Longrightarrow> P"
+   \<And>v. A,\<Gamma> \<turnstile> \<langle>e, n_s\<rangle> \<Down> v \<Longrightarrow> s' = Normal (n_s(x \<mapsto> v)) \<Longrightarrow> P \<rbrakk> \<Longrightarrow> P"
   apply (erule red_cmd.cases; simp)
   apply (erule red_exprs.cases; simp)
   by auto
 
 lemma havoc_cases:
-  "\<lbrakk>\<Lambda>,\<Gamma> \<turnstile> \<langle>Havoc x, s\<rangle> \<rightarrow> s';
+  "\<lbrakk>A,\<Lambda>,\<Gamma> \<turnstile> \<langle>Havoc x, s\<rangle> \<rightarrow> s';
     s = Normal n_s;
     map_of \<Lambda> x = Some ty;
-    \<And>v. type_of_val v = ty \<Longrightarrow> s' = Normal (n_s(x \<mapsto> v)) \<Longrightarrow> P\<rbrakk> \<Longrightarrow> P"
-  by (erule red_cmd.cases; simp)
+    \<And>v. ty_val_rel A v ty \<Longrightarrow> s' = Normal (n_s(x \<mapsto> v)) \<Longrightarrow> P\<rbrakk> \<Longrightarrow> P"
+  by (erule red_cmd.cases; simp) 
 
 lemma type_of_val_int_elim:
-  "\<lbrakk> type_of_val v = TInt;
-     \<And>i. v = IntV i \<Longrightarrow> P
+  "\<lbrakk> ty_val_rel A v (TPrim TInt);
+     \<And>i. v = LitV (LInt i) \<Longrightarrow> P
    \<rbrakk> \<Longrightarrow> P"
-  by (cases v; auto)
+  apply (cases v)
+   apply auto[2]
+  by (metis lit.exhaust prim_ty.distinct(1) type_of_lit.simps(1))
 
 lemma type_of_val_bool_elim:
-  "\<lbrakk> type_of_val v = TBool;
-     \<And>b. v = BoolV b \<Longrightarrow> P
+  "\<lbrakk> ty_val_rel A v (TPrim TBool);
+     \<And>b. v = LitV (LBool b) \<Longrightarrow> P
    \<rbrakk> \<Longrightarrow> P"
-  by (cases v; auto)
+  apply (cases v)
+   apply auto[2]
+  by (metis lit.exhaust prim_ty.distinct(1) type_of_lit.simps(2))
 
+ 
 lemma val_elim [elim!]:
- "\<lbrakk> \<Gamma> \<turnstile> \<langle>Val v, n_s\<rangle> \<Down> v'; v = v' \<Longrightarrow> P \<rbrakk> \<Longrightarrow> P"
+ "\<lbrakk> A,\<Gamma> \<turnstile> \<langle>Lit l, n_s\<rangle> \<Down> v'; (LitV l) = v' \<Longrightarrow> P \<rbrakk> \<Longrightarrow> P"
   by (erule red_expr.cases; simp)
 
 lemma cons_exp_elim :
- "\<Gamma> \<turnstile> \<langle>e # es, n_s\<rangle> [\<Down>] vs \<Longrightarrow> (vs \<noteq> [] \<Longrightarrow> \<Gamma> \<turnstile> \<langle>e, n_s\<rangle> \<Down> hd vs \<Longrightarrow> \<Gamma> \<turnstile> \<langle>es, n_s\<rangle> [\<Down>] tl vs \<Longrightarrow> P) \<Longrightarrow> P"
+ "A,\<Gamma> \<turnstile> \<langle>e # es, n_s\<rangle> [\<Down>] vs \<Longrightarrow> (vs \<noteq> [] \<Longrightarrow> A,\<Gamma> \<turnstile> \<langle>e, n_s\<rangle> \<Down> hd vs \<Longrightarrow> A,\<Gamma> \<turnstile> \<langle>es, n_s\<rangle> [\<Down>] tl vs \<Longrightarrow> P) \<Longrightarrow> P"
   by (erule red_exprs.cases; simp_all)
 
 lemma cons_exp_elim2:
-  "\<lbrakk>\<Gamma> \<turnstile> \<langle>e # es, n_s\<rangle> [\<Down>] vs;
-   \<And>v vs'. vs = v # vs' \<Longrightarrow> \<Gamma> \<turnstile> \<langle>e, n_s\<rangle> \<Down> v \<Longrightarrow> \<Gamma> \<turnstile> \<langle>es, n_s\<rangle> [\<Down>] vs' \<Longrightarrow> P\<rbrakk> \<Longrightarrow> P" 
+  "\<lbrakk>A,\<Gamma> \<turnstile> \<langle>e # es, n_s\<rangle> [\<Down>] vs;
+   \<And>v vs'. vs = v # vs' \<Longrightarrow> A,\<Gamma> \<turnstile> \<langle>e, n_s\<rangle> \<Down> v \<Longrightarrow> A,\<Gamma> \<turnstile> \<langle>es, n_s\<rangle> [\<Down>] vs' \<Longrightarrow> P\<rbrakk> \<Longrightarrow> P" 
   by (erule red_exprs.cases; simp_all)
 
 lemma singleton_exp:
-  "\<Gamma> \<turnstile> \<langle>[e], n_s\<rangle> [\<Down>] vs \<Longrightarrow> \<Gamma> \<turnstile> \<langle>e, n_s\<rangle> \<Down> hd vs"
+  "A,\<Gamma> \<turnstile> \<langle>[e], n_s\<rangle> [\<Down>] vs \<Longrightarrow> A,\<Gamma> \<turnstile> \<langle>e, n_s\<rangle> \<Down> hd vs"
   by (auto elim: cons_exp_elim)
 
 lemma nil_exp_elim [elim!]:
- "\<lbrakk>\<Gamma> \<turnstile> \<langle>[], n_s\<rangle> [\<Down>] vs; vs = [] \<Longrightarrow> P\<rbrakk> \<Longrightarrow> P"
+ "\<lbrakk>A,\<Gamma> \<turnstile> \<langle>[], n_s\<rangle> [\<Down>] vs; vs = [] \<Longrightarrow> P\<rbrakk> \<Longrightarrow> P"
  by (erule red_exprs.cases; simp)
 
 
 lemma nil_cmd_elim [elim!]:
- "\<lbrakk>\<Lambda>,\<Gamma> \<turnstile> \<langle>[], s\<rangle> [\<rightarrow>] s'; s' = s \<Longrightarrow> P\<rbrakk> \<Longrightarrow> P"
+ "\<lbrakk>A,\<Lambda>,\<Gamma> \<turnstile> \<langle>[], s\<rangle> [\<rightarrow>] s'; s' = s \<Longrightarrow> P\<rbrakk> \<Longrightarrow> P"
   by (erule red_cmd_list.cases; simp)
 
 lemma magic_stays_cmd_list_2:
-  assumes "\<Lambda>,\<Gamma> \<turnstile> \<langle>cs, s\<rangle> [\<rightarrow>] s'" and "s = Magic"
+  assumes "A,\<Lambda>,\<Gamma> \<turnstile> \<langle>cs, s\<rangle> [\<rightarrow>] s'" and "s = Magic"
   shows   "s' = Magic"
   using assms
   by (simp add: magic_stays_cmd_list)
